try proving flen_ok using the new interface

src/File.v
@@ -82,6 +82,12 @@ Module FILE.
      [[ length ilist = length flist ]] *
      listpred file_match (combine ilist flist))%pred.
 
+  Definition inum_valid inum ixp (flist : list file) :=
+      (inum < IXLen ixp ^* INODE.items_per_valu)%word /\
+      wordToNat inum < length flist.
+
+  Definition off_valid (off : addr) f :=
+    wordToNat off < length (FData f).
 
 
   (* correctness theorems *)
@@ -89,7 +95,7 @@ Module FILE.
   Theorem fread_ok : forall lxp bxp ixp inum off,
     {<F A B mbase m flist f v,
     PRE    LOG.rep lxp (ActiveTxn mbase m) *
-           [[ wordToNat inum < length flist /\ wordToNat off < length (FData f) ]] *
+           [[ inum_valid inum ixp flist /\ off_valid off f ]] *
            [[ (F * rep bxp ixp flist)%pred m ]] *
            [[ (A * inum |-> f)%pred (list2mem flist) ]] *
            [[ (B * off |-> v)%pred (list2mem (FData f)) ]]
@@ -104,7 +110,7 @@ Module FILE.
   Lemma fwrite_ok : forall lxp bxp ixp inum off v,
     {<F A B mbase m flist f v0,
     PRE    LOG.rep lxp (ActiveTxn mbase m) *
-           [[ wordToNat inum < length flist /\ wordToNat off < length (FData f) ]] *
+           [[ inum_valid inum ixp flist /\ off_valid off f ]] *
            [[ (F * rep bxp ixp flist)%pred m ]] *
            [[ (A * inum |-> f)%pred (list2mem flist) ]] *
            [[ (B * off |-> v0)%pred (list2mem (FData f)) ]]
@@ -124,7 +130,7 @@ Module FILE.
   Theorem flen_ok : forall lxp bxp ixp inum,
     {< F A mbase m flist f,
     PRE    LOG.rep lxp (ActiveTxn mbase m) *
-           [[ wordToNat inum < length flist ]] *
+           [[ inum_valid inum ixp flist ]] *
            [[ (F * rep bxp ixp flist)%pred m ]] *
            [[ (A * inum |-> f)%pred (list2mem flist) ]]
     POST:r LOG.rep lxp (ActiveTxn mbase m) *
@@ -132,14 +138,37 @@ Module FILE.
     CRASH  LOG.log_intact lxp mbase
     >} flen lxp ixp inum.
   Proof.
+    unfold flen, rep, file_match, inum_valid.
+    hoare.
+
+    instantiate (a3 := l0).
+    unfold INODE.inum_valid; intuition.
+    cancel.
+
+    (* Automation should be able to figure out what is ?a4.
+       We also need to construct frame ?a0, the predicate about all other
+       items in the list.  We can do so via array_isolate.
+       But why do we have to?  All other items are totally irrelevant.
+       Maybe separation logic is not good for lists?
+     *)
     admit.
+
+    instantiate (a4 := (sel l0 inum INODE.inode0)).
+    rewrite listpred_extract with (i := wordToNat inum) (def := (INODE.inode0, file0)) in H5.
+    autorewrite with core in H5; auto.
+    simpl in H5; auto.
+    destruct_lift H5.
+    subst; f_equal.
+    apply list2mem_sel with (def:=file0) in H4; auto.
+    unfold sel; subst; auto.
+    rewrite combine_length_eq; try omega. 
   Qed.
 
 
   Theorem fgrow_ok : forall lxp bxp ixp inum,
     {< F A mbase m flist f,
     PRE    LOG.rep lxp (ActiveTxn mbase m) *
-           [[ wordToNat inum < length flist ]] *
+           [[ inum_valid inum ixp flist ]] *
            [[ length (FData f) < INODE.blocks_per_inode ]] *
            [[ (F * rep bxp ixp flist)%pred m ]] *
            [[ (A * inum |-> f)%pred (list2mem flist) ]]
@@ -159,7 +188,7 @@ Module FILE.
   Theorem fshrink_ok : forall lxp bxp ixp inum,
     {< F A mbase m flist f,
     PRE    LOG.rep lxp (ActiveTxn mbase m) *
-           [[ wordToNat inum < length flist /\ length (FData f) > 0 ]] *
+           [[ inum_valid inum ixp flist /\ length (FData f) > 0 ]] *
            [[ (F * rep bxp ixp flist)%pred m ]] *
            [[ (A * inum |-> f)%pred (list2mem flist) ]]
     POST:r [[ r = false ]] * (exists m', LOG.rep lxp (ActiveTxn mbase m')) \/
